examples/t2/P26.v
@@ -1,0 +1,130 @@
+
+From CTree Require Import
+  CTree.Core
+  Events.State
+  Events.Writer
+  Logic.Ctl
+  CTree.Equ
+  CTree.SBisim
+  CTree.Logic.Trans
+  Logic.Kripke
+  CTree.Interp.Core
+  CTree.Logic.AF
+  CTree.Logic.AX
+  CTree.Logic.Bind
+  CTree.Logic.Iter
+  CTree.Logic.State
+  CTree.Logic.CanStep
+  CTree.Interp.State
+  CTree.Events.State
+  CTree.Events.Writer
+  Lang.Clang.
+
+From ExtLib Require Import
+  String
+  Data.Map.FMapAList
+  Structures.Maps.
+
+From Coq Require Import
+  Strings.String
+  Lia
+  ZArith.
+
+Generalizable All Variables.
+
+Import Ctree CTreeNotations CtlNotations.
+Local Open Scope ctl_scope.
+Local Open Scope ctree_scope.
+Local Open Scope Z_scope.
+
+(*
+void main() {
+
+    int varC; // assume varC >= 1
+    int varR = 0;
+    int varCS = 4;
+
+
+    while (varCS > 0) {
+        if (varC >= varCS) {
+            varC = varC - 1;
+            varR = varR + 1;
+            varCS = varCS - 1;
+        } else {
+            /* varC = varC - 1; */ 
+            /* varR = varR + 1; */ 
+            varCS = varCS - 1;
+        }
+    }
+}
+ *)
+
+Module P26.
+  Include Clang.Clang.
+  Local Open Scope clang_scope.
+
+  Definition c: string := "c".
+  Definition r: string := "r".
+  Definition cs: string := "cs".
+  
+  Definition p26: CProg :=
+    [[
+        r := 0 ;;;
+        cs := 4 ;;;
+        while cs > 0 do
+          if c >= cs then
+            c := c - 1 ;;;
+            r := r + 1 ;;;
+            cs := cs - 1
+          else
+            cs := cs - 1
+    ]].
+
+  Arguments alist_add /.
+
+  (* // (varC > 5) || [EG](varR <= 5) *)
+  Lemma p26_spec: forall cval,
+      let init := add r 0 (add c cval empty) in
+      <( {instr_cprog p26 init}, {Obs (Log init) tt} |=
+           (visW {assert c (fun cv => cv > 5)} \/ EG visW {assert r (fun rv => rv <= 5)}) )>.
+  Proof with eauto with ctl.
+    intros.
+    unfold p26, init.
+    destruct (Z.le_gt_cases cval 5).
+    - cright. (* cv <= 5 *)      
+      eapply eg_cprog_seq.
+      + eapply eur_cprog_assgn_eq...
+        constructor; cbn; lia.
+      + eapply eg_cprog_seq.
+        * eapply eur_cprog_assgn_eq...
+          constructor; cbn; lia.
+        * cbn.
+          (* unfolding doesn't work, need [eg_iter] lemma *)
+          eapply eg_cprog_while_gt with
+            (R:=fun ctx => ctx = ((cs, 3) :: (r, 1) :: (c, cval - 1) :: nil)%list \/
+                          ctx = ((cs, 4) :: (r, 0) :: (c, cval) :: nil)%list)...
+          -- right; reflexivity. cbn; lia.
+          -- eapply eur_cprog_ite_gte; cbn.
+             pose proof (Zge_cases cval 4); destruct (cval >=? 4).
+             ++ eapply eur_cprog_seq.
+                ** eapply eur_cprog_assgn_eq...
+                   constructor; cbn; lia.
+                ** eapply eur_cprog_seq.
+                   --- eapply eur_cprog_assgn_eq...
+                       constructor; cbn; lia.
+                   --- cbn.
+                       eapply eur_cprog_assgn...
+                       +++ constructor; cbn; lia.
+             ++ eapply eur_cprog_assgn...
+                constructor; cbn; lia.
+          -- intros ctx [-> | ->].
+             ++ 
+      + eapply aul_cprog_seq.
+        * eapply afr_cprog_assgn...
+          eapply axr_cexp_const...
+        * do 7 p25_unfold.
+          cleft.
+          apply vis_c_assert... *)
+  Qed.
+
+End P25.        
